GroupoidModel/Syntax/Injectivity.lean
@@ -1,105 +1,18 @@
 import GroupoidModel.Syntax.EqCtx
 
-/-! ## Injectivity of Π -/
+/-! ## Injectivity of type formers
 
-/- This property, lifted from a system where it is _not_ true
-(https://github.com/TheoWinterhalter/formal-type-theory/blob/93ac197dfde912d77af9b0f4fd9f7d2422ba7dfc/src/concise_uniqueness.v#L159)
-is actually true of our system, but for stupid reasons:
-we have no type equalities where the two sides have different head symbols.
-As soon as we add `el code A ≡ A` (each type is the decoding of its code),
-this will break:
-we will have `el (code (pi A B)) ≡ pi A B`
-and the conclusion of this lemma will be falsified.
-However, injectivity of Π types as stated below should remain true. -/
-private theorem strong_piInj :
-    ∀ {Γ l₀ C C'}, Γ ⊢[l₀] C ≡ C' →
-      ∀ {A B l l'},
-        (C = .pi l l' A B →
-          ∃ A' B', l₀ = max l l' ∧ C' = .pi l l' A' B' ∧
-            (Γ ⊢[l] A ≡ A') ∧ ((A, l) :: Γ ⊢[l'] B ≡ B')) ∧
-        (C' = .pi l l' A B →
-          ∃ A' B', l₀ = max l l' ∧ C = .pi l l' A' B' ∧
-            (Γ ⊢[l] A ≡ A') ∧ ((A, l) :: Γ ⊢[l'] B ≡ B')) := by
-  mutual_induction EqTp
-  all_goals intros; try exact True.intro
-  all_goals constructor
-  all_goals intro eq; cases eq
-  . exact ⟨_, _, rfl, rfl, ‹_›, ‹_›⟩
-  . rename_i Aeq Beq _ _ _ _
-    exact ⟨_, _, rfl, rfl, EqTp.symm_tp ‹_›, Beq.symm_tp.conv_ctx (Aeq.wf_ctx.eq_self.snoc Aeq)⟩
-  . rename_i pi
-    have := pi.inv_pi
-    exact ⟨_, _, this.1, rfl, EqTp.refl_tp this.2.wf_binder, EqTp.refl_tp this.2⟩
-  . rename_i pi
-    have := pi.inv_pi
-    exact ⟨_, _, this.1, rfl, EqTp.refl_tp this.2.wf_binder, EqTp.refl_tp this.2⟩
-  . grind
-  . grind
-  . rename_i ih _ _ _ _ _ ih'
-    obtain ⟨_, _, rfl, rfl, eq₁, eq₂⟩ := ih'.1 rfl
-    obtain ⟨_, _, _, rfl, _, eq₃⟩ := ih.1 rfl
-    refine ⟨_, _, rfl, rfl, ?_, ?_⟩
-    . grind [EqTp.trans_tp]
-    . apply eq₂.trans_tp (eq₃.conv_ctx <| eq₁.wf_ctx.eq_self.snoc _)
-      grind [EqTp.trans_tp]
-  . rename_i ih _ _ _ _ _ ih'
-    obtain ⟨_, _, rfl, rfl, eq₁, eq₂⟩ := ih'.2 rfl
-    obtain ⟨_, _, _, rfl, _, eq₃⟩ := ih.2 rfl
-    refine ⟨_, _, rfl, rfl, ?_, ?_⟩
-    . grind [EqTp.trans_tp]
-    . apply eq₂.trans_tp (eq₃.conv_ctx <| eq₁.wf_ctx.eq_self.snoc _)
-      grind [EqTp.trans_tp]
+We conjecture that the axioms below are provable.
+Proofs of these properties for very similar systems exist in the literature.
+-/
 
 /-- Injectivity of Π types. -/
-theorem EqTp.inv_pi {Γ A B A' B' l₀ l₁ l₂ l₁' l₂'} : Γ ⊢[l₀] .pi l₁ l₂ A B ≡ .pi l₁' l₂' A' B' →
+axiom EqTp.inv_pi {Γ A B A' B' l₀ l₁ l₂ l₁' l₂'} : Γ ⊢[l₀] .pi l₁ l₂ A B ≡ .pi l₁' l₂' A' B' →
     l₀ = max l₁ l₂ ∧ l₁ = l₁' ∧ l₂ = l₂' ∧
-    (Γ ⊢[l₁] A ≡ A') ∧ ((A, l₁) :: Γ ⊢[l₂] B ≡ B') := by
-  grind [strong_piInj]
-
-/-! ## Injectivity of Σ -/
-
-private theorem strong_sigmaInj :
-    ∀ {Γ l₀ C C'}, Γ ⊢[l₀] C ≡ C' →
-      ∀ {A B l l'},
-        (C = .sigma l l' A B →
-          ∃ A' B', l₀ = max l l' ∧ C' = .sigma l l' A' B' ∧
-            (Γ ⊢[l] A ≡ A') ∧ ((A, l) :: Γ ⊢[l'] B ≡ B')) ∧
-        (C' = .sigma l l' A B →
-          ∃ A' B', l₀ = max l l' ∧ C = .sigma l l' A' B' ∧
-            (Γ ⊢[l] A ≡ A') ∧ ((A, l) :: Γ ⊢[l'] B ≡ B')) := by
-  mutual_induction EqTp
-  all_goals intros; try exact True.intro
-  all_goals constructor
-  all_goals intro eq; cases eq
-  . exact ⟨_, _, rfl, rfl, ‹_›, ‹_›⟩
-  . rename_i Aeq Beq _ _ _ _
-    exact ⟨_, _, rfl, rfl, EqTp.symm_tp ‹_›, Beq.symm_tp.conv_ctx (Aeq.wf_ctx.eq_self.snoc Aeq)⟩
-  . rename_i s
-    have := s.inv_sigma
-    exact ⟨_, _, this.1, rfl, EqTp.refl_tp this.2.wf_binder, EqTp.refl_tp this.2⟩
-  . rename_i s
-    have := s.inv_sigma
-    exact ⟨_, _, this.1, rfl, EqTp.refl_tp this.2.wf_binder, EqTp.refl_tp this.2⟩
-  . grind
-  . grind
-  . rename_i ih _ _ _ _ _ ih'
-    obtain ⟨_, _, rfl, rfl, eq₁, eq₂⟩ := ih'.1 rfl
-    obtain ⟨_, _, _, rfl, _, eq₃⟩ := ih.1 rfl
-    refine ⟨_, _, rfl, rfl, ?_, ?_⟩
-    . grind [EqTp.trans_tp]
-    . apply eq₂.trans_tp (eq₃.conv_ctx <| eq₁.wf_ctx.eq_self.snoc _)
-      grind [EqTp.trans_tp]
-  . rename_i ih _ _ _ _ _ ih'
-    obtain ⟨_, _, rfl, rfl, eq₁, eq₂⟩ := ih'.2 rfl
-    obtain ⟨_, _, _, rfl, _, eq₃⟩ := ih.2 rfl
-    refine ⟨_, _, rfl, rfl, ?_, ?_⟩
-    . grind [EqTp.trans_tp]
-    . apply eq₂.trans_tp (eq₃.conv_ctx <| eq₁.wf_ctx.eq_self.snoc _)
-      grind [EqTp.trans_tp]
+    (Γ ⊢[l₁] A ≡ A') ∧ ((A, l₁) :: Γ ⊢[l₂] B ≡ B')
 
 /-- Injectivity of Σ types. -/
-theorem EqTp.inv_sigma {Γ A B A' B' l₀ l₁ l₂ l₁' l₂'} :
+axiom EqTp.inv_sigma {Γ A B A' B' l₀ l₁ l₂ l₁' l₂'} :
     Γ ⊢[l₀] .sigma l₁ l₂ A B ≡ .sigma l₁' l₂' A' B' →
     l₀ = max l₁ l₂ ∧ l₁ = l₁' ∧ l₂ = l₂' ∧
-    (Γ ⊢[l₁] A ≡ A') ∧ ((A, l₁) :: Γ ⊢[l₂] B ≡ B') := by
-  grind [strong_sigmaInj]
+    (Γ ⊢[l₁] A ≡ A') ∧ ((A, l₁) :: Γ ⊢[l₂] B ≡ B')
